src/goose_lang/ffi/grove_filesys_axioms.v
@@ -2,26 +2,10 @@ From Perennial.goose_lang Require Export prelude ffi.grove_prelude.
 From Perennial.goose_lang Require Export lang.
 From iris.base_logic Require Import ghost_map.
 From Perennial.program_proof Require Import proof_prelude.
-From Perennial.goose_lang Require Export prelude ffi.grove_ffi.
-
-Class filesysG Σ := FileSysG {
-  filesys_gname : gname ; (* Name of str -> []byte authmap used for filesys ffi *)
-  filesys_inG :> ghost_mapG Σ string (list byte)
-}.
+From Perennial.goose_lang Require Export prelude ffi.grove_prelude.
 
 Section filesys.
 Context `{!heapGS Σ}.
-
-Definition file_mapsto {fG:filesysG Σ} (s:string) (c:list byte) (dq:dfrac): iProp Σ :=
-  s ↪[filesys_gname]{dq} c.
-
-Notation "s f↦{ q } c" := (file_mapsto s c q)
-(at level 20, q at level 50, format "s  f↦{ q } c") : bi_scope.
-
-Notation "s f↦ c" := (s f↦{DfracOwn 1} c)%I
-(at level 20, format "s  f↦ c") : bi_scope.
-
-Context `{!filesysG Σ}.
 
 Axiom wpc_Read : ∀ filename (dq:dfrac) content,
   {{{
@@ -67,9 +51,3 @@ Axiom wpc_AtomicAppend : ∀ filename content_old content (content_sl:Slice.t) q
   }}}.
 
 End filesys.
-
-Notation "s f↦{ q } c" := (file_mapsto s c q)
-(at level 20, q at level 50, format "s  f↦{ q } c") : bi_scope.
-
-Notation "s f↦ c" := (s f↦{DfracOwn 1} c)%I
-(at level 20, format "s  f↦ c") : bi_scope.
